src/SeqDisk/ReplicatedDisk/ReadWrite.v
@@ -57,7 +57,7 @@ Section ReplicatedDiskReadWrite.
            |})
         (Read a)
         (irec td)
-        (refinement td).
+        (interface_abs td).
   Proof.
     unfold Read.
 
@@ -91,7 +91,7 @@ Section ReplicatedDiskReadWrite.
            |})
         (Write a b)
         (irec td)
-        (refinement td).
+        (interface_abs td).
   Proof.
     unfold Write.
 
